Improving Factorial example

platform/cito/examples/Factorial.v
@@ -14,115 +14,16 @@ Require Import Arith.
 
 Definition fact_w (w : W) := natToW (fact (wordToNat w)).
 
-Fixpoint fact_partial' start n :=
-  match n with
-    | 0 => 1
-    | S n' => start * fact_partial' (1 + start) n'
-  end.
-
-(* (a+1) * (a+2) * ... * b  (1 when a>=b) *)
-Definition fact_partial (a b : nat) := fact_partial' (1 + a) (b - a).
-
-Definition fact_partial_w (a b : W) : W := natToW (fact_partial (wordToNat a) (wordToNat b)).
-
-Set Printing Coercions.
-
-Lemma fact_partial_0 : forall n, fact_partial 0 n = fact n.
-  unfold fact_partial.
-  induction n; simpl; intuition.
-  rewrite plus_0_r in *.
-  Require Import NPeano.
-  Import NPeano.Nat.
-  rewrite sub_0_r in *.
-  Lemma fact_partial'_inv : forall n start, fact_partial' start n * (n + start) = start * fact_partial' (1 + start) n.
-    Opaque mult.
-    induction n; simpl; intuition.
-    repeat rewrite <- IHn.
-    rewrite mult_assoc.
-    repeat rewrite <- IHn.
-    ring.
-    Transparent mult.
-  Qed.
-  specialize (fact_partial'_inv n 1); intro; simpl in *.
-  rewrite plus_0_r in *.
-  rewrite <- H.
-  rewrite IHn.
-  ring.
-Qed.
-
-Lemma fact_partial_w_0 : forall w, fact_partial_w $0 w = fact_w w.
-  intros.
-  unfold fact_partial_w, fact_w.
-  f_equal.
-  change (wordToNat $0) with 0.
-  eapply fact_partial_0.
-Qed.
-
-Lemma fact_partial_w_same : forall w, fact_partial_w w w = 1.
-  intros.
-  unfold fact_partial_w.
-  f_equal.
-  unfold fact_partial.
-  rewrite minus_diag.
-  simpl; eauto.
-Qed.
-
-Lemma fact_partial_update : forall a b, 0 < a -> a <= b -> a * fact_partial a b = fact_partial (a - 1) b.
-  intros.
-  unfold fact_partial.
-  Opaque mult.
-  simpl.
-  replace (b - (a - 1)) with (S (b - a)).
-  replace (S (a - 1)) with a.
-  simpl.
-  eauto.
-  omega.
-  omega.
-  Transparent mult.
-Qed.
-
-Require Import WordFacts WordFacts2 WordFacts3 WordFacts4.
-Require Import GeneralTactics2.
-
-Lemma wmult_natToW_comm : forall a b, $ a ^* $ b = natToW (a * b).
-  symmetry.
-  eapply natToWord_mult.
-Qed.
-
-Lemma fact_partial_w_update : forall (a b : W), ($0 < a -> a <= b -> a ^* fact_partial_w a b = fact_partial_w (a ^- $1) b)%word.
-  unfold fact_partial_w.
-  intros.
-  set (wordToNat a).
-  set (wordToNat (_ ^- _)).
-  replace a with (natToW (wordToNat a)).
-  rewrite wmult_natToW_comm.
-  f_equal.
-  subst n n0.
-  replace (wordToNat (_ ^- _)) with (wordToNat a - 1).
-  eapply fact_partial_update.
-  nomega.
-  nomega.
-  Focus 2.
-  eapply natToWord_wordToNat.
-  rewrite wordToNat_wminus.
-  rewrite roundTrip_1.
-  eauto.
-  eapply non_zero_wge1.
-  nintro.
-  subst.
-  nomega.
-Qed.
-
 Import ProgramLogicMake.
 
 Definition body := (
-    "ret" <- 1 ;;
-    [ fun v0 v => 
-        sel (fst v) "ret" = fact_partial_w (sel (fst v) "n") (sel (fst v0) "n") /\ 
-        (sel (fst v) "n" <= sel (fst v0) "n")%word /\
-        snd v = snd v0 ]
+    "ret" <- 1;;
+    [BEFORE(V, h)
+     AFTER(V', h')
+       fact_w (V "n") = V' "ret" ^* fact_w (V' "n")
+       /\ h' = h]
     While (0 < "n") {
-      "ret" <- "ret" * "n" ;;
+      "ret" <- "ret" * "n";;
       "n" <- "n" - 1                          
     }
   )%stmtex.
@@ -170,117 +71,52 @@ Definition top := bimport [[ ("fact"!"fact", fspec), "sys"!"printInt" @ [printIn
     end
   }}.
 
-Import LinkSpecMake.
-
-Open Scope word.
-
-Lemma wle_0_eq : forall w : W, w <= $0 -> w = $0.
-  intros.
-  unfold wlt in *.
-  destruct (N.eq_0_gt_0_cases (wordToN w)).
-  change (0)%N with (wordToN (natToW 0)) in H0.
-  eapply wordToN_inj in H0.
-  eauto.
-  change (wordToN ($ 0)) with 0%N in H.
-  intuition.
-Qed.
-
-Lemma sel_upd_eq' : forall vs nm v nm', nm = nm' -> (upd vs nm v) nm' = v.
-  intros; eapply sel_upd_eq; eauto.
-Qed.
-
-Lemma sel_upd_ne' : forall vs nm v nm', nm <> nm' -> (upd vs nm v) nm' = sel vs nm'.
-  intros; eapply sel_upd_ne; eauto.
-Qed.
-
-Ltac sel_upd_simpl :=
-  repeat 
-    match goal with
-      | H : _ |- _ => rewrite sel_upd_eq in H by reflexivity
-      | H : _ |- _ => rewrite sel_upd_ne in H by discriminate
-      | |- _ => rewrite sel_upd_eq by reflexivity
-      | |- _ => rewrite sel_upd_ne by discriminate
-      | H : _ |- _ => rewrite sel_upd_eq' in H by reflexivity
-      | H : _ |- _ => rewrite sel_upd_ne' in H by discriminate
-      | |- _ => rewrite sel_upd_eq' by reflexivity
-      | |- _ => rewrite sel_upd_ne' by discriminate
-    end.
-
-Lemma is_true_0_lt : forall v v' (x : string), is_true (0 < x)%expr v v' -> $0 < sel (fst v') x.
-  intros.
-  unfold is_true, abs in *.
-  simpl in *.
-  unfold wltb in *.
-  destruct (wlt_dec _ _).
-  eauto.
-  intuition.
-Qed.
-
 Definition empty_precond : assert := fun v0 v => v0 = v.
 
-Lemma vcs_good : and_all (vc body empty_precond).
-  unfold body, empty_precond; simpl.
-  unfold imply_close, and_lift, interp, abs; simpl.
-  descend.
-  openhyp.
-  subst.
-  simpl.
-  split.
-  rewrite sel_upd_ne by eauto.
-  rewrite H0.
-  symmetry; eapply fact_partial_w_same.
-  eauto.
-  openhyp; simpl in *.
-  destruct v; destruct v'; simpl in *.
-  sel_upd_simpl.
-  subst.
-  eapply is_true_0_lt in H2.
-  simpl in *.
-  sel_upd_simpl.
-  split.
-  rewrite H1.
-  rewrite H0.
-  rewrite <- fact_partial_w_update.
-  words.
-  eauto.
-  eauto.
-  split.
-  rewrite H0.
-  nomega.
-  eauto.
-  eauto.
+Require Import WordFacts2 WordFacts5.
+
+Lemma fact_step : forall n,
+  ($0 < n)%word
+  -> fact_w n = n ^* fact_w (n ^- $1).
+  intros.
+  unfold fact_w.
+  rewrite wordToNat_positive by assumption.
+  unfold fact at 1; fold fact.
+  rewrite <- wordToNat_positive by assumption.
+  unfold natToW; rewrite natToWord_mult.
+  rewrite natToWord_wordToNat.
+  reflexivity.
 Qed.
 
+Hint Rewrite fact_step using solve [ eauto 2 ] : sepFormula.
+
+Lemma vcs_good : and_all (vc body empty_precond).
+  unfold empty_precond; cito_vcs body; words.
+Qed.
+
+Local Hint Immediate vcs_good.
+
+Theorem final : forall n x r,
+  ($0 >= n)%word
+  -> x = r ^* fact_w n
+  -> r = x.
+  intros; subst.
+  assert (n = $0) by (apply wordToNat_inj; nomega).
+  subst.
+  change (fact_w $0) with (natToW 1).
+  words.
+Qed.
+
+Local Hint Resolve final.
+
+Import LinkSpecMake.
+
 Lemma body_runsto : forall stn fs v v', stn_good_to_use (gm :: nil) (empty _) stn -> fs_good_to_use (gm :: nil) (empty _) fs stn -> RunsTo (from_bedrock_label_map (Labels stn), fs stn) (Body f) v v' -> sel (fst v') (RetVar f) = fact_w (sel (fst v) "n") /\ snd v' = snd v.
-  intros.
-  unfold f in *; simpl in *.
-  eapply sound_runsto' with (p := empty_precond) in H1.
-  2 : instantiate (1 := body); simpl; eauto.
-  simpl in *.
-  unfold and_lift, interp, abs in *.
-  openhyp.
-  split.
-  2 : eauto.
-  rewrite H1.
-  replace (sel (fst v') "n") with (natToW 0).
-  eapply fact_partial_w_0.
-  unfold is_false, abs in *; simpl in *.
-  unfold wltb in *.
-  destruct wlt_dec; try discriminate.
-  symmetry.
-  eapply wle_0_eq; eauto.
-  eapply vcs_good.
-  unfold interp, empty_precond; eauto.
+  cito_runsto f empty_precond; eauto.
 Qed.
 
 Lemma body_safe : forall stn fs v, stn_good_to_use (gm :: nil) (empty _) stn -> fs_good_to_use (gm :: nil) (empty _) fs stn -> Safe (from_bedrock_label_map (Labels stn), fs stn) (Body f) v.
-  intros.
-  unfold f in *; simpl in *.
-  eapply sound_safe with (p := empty_precond).
-  instantiate (1 := body).
-  eauto.
-  eapply vcs_good.
-  unfold interp, empty_precond; eauto.
+  cito_safe f body empty_precond.
 Qed.
 
 Require Import Inv.
